More progress on generic reflective ops
Add hlistP

More work towards generic reflective lemmas

Work towards reasonable interpretations

src/Specific/GF25519Reflective/Common.v
@@ -11,6 +11,7 @@ Require Import Crypto.Reflection.Z.Reify.
 Require Export Crypto.Reflection.Z.Syntax.
 Require Import Crypto.Reflection.InterpWfRel.
 Require Import Crypto.Reflection.Application.
+Require Import Crypto.Reflection.ApplicationLemmas.
 Require Import Crypto.Reflection.MapInterp.
 Require Import Crypto.Reflection.MapInterpWf.
 Require Import Crypto.Reflection.WfReflective.
@@ -140,16 +141,69 @@ Definition Expr9Op_bounds : interp_all_binders_for Expr9_4OpT ZBounds.interp_bas
 Definition ExprUnOpWireToFE_bounds : interp_all_binders_for ExprUnOpWireToFET ZBounds.interp_base_type.
 Proof. make_bounds (Tuple.to_list _ wire_digit_bounds). Defined.
 
-Definition interp_bexpr : ExprBinOp -> Specific.GF25519BoundedCommon.fe25519W -> Specific.GF25519BoundedCommon.fe25519W -> Specific.GF25519BoundedCommon.fe25519W
-  := fun e => curry_binop_fe25519W (Interp (@WordW.interp_op) e).
-Definition interp_uexpr : ExprUnOp -> Specific.GF25519BoundedCommon.fe25519W -> Specific.GF25519BoundedCommon.fe25519W
-  := fun e => curry_unop_fe25519W (Interp (@WordW.interp_op) e).
-Definition interp_uexpr_FEToZ : ExprUnOpFEToZ -> Specific.GF25519BoundedCommon.fe25519W -> Specific.GF25519BoundedCommon.word64
-  := fun e => curry_unop_fe25519W (Interp (@WordW.interp_op) e).
-Definition interp_uexpr_FEToWire : ExprUnOpFEToWire -> Specific.GF25519BoundedCommon.fe25519W -> Specific.GF25519BoundedCommon.wire_digitsW
-  := fun e => curry_unop_fe25519W (Interp (@WordW.interp_op) e).
-Definition interp_uexpr_WireToFE : ExprUnOpWireToFE -> Specific.GF25519BoundedCommon.wire_digitsW -> Specific.GF25519BoundedCommon.fe25519W
-  := fun e => curry_unop_wire_digitsW (Interp (@WordW.interp_op) e).
+Fixpoint interp_of_tower count_in count_out
+  : tower_nd Z (interp_flat_type interp_base_type (Expr_n_OpT count_out)) (count_in * length_fe25519)
+    -> interp_type_gen (interp_flat_type interp_base_type) (Expr_nm_OpT count_in count_out).
+Proof.
+  refine match count_in
+               return tower_nd Z _ (count_in * length_fe25519)
+                      -> interp_type_gen (interp_flat_type interp_base_type) (Expr_nm_OpT count_in count_out)
+         with
+         | 0 => fun x => x
+         | S n => _
+         end.
+  simpl.
+  intro f.
+  repeat let x := fresh "x" in intro x; specialize (f x).
+  exact (@interp_of_tower n count_out f).
+Defined.
+
+Definition uninterp_of_tower {T} count_in count_out
+  : tower_nd T (interp_flat_type interp_base_type (Expr_n_OpT count_out)) count_in
+    -> tower_nd T (Tuple.tuple GF25519.fe25519 count_out) count_in
+  := impl_under_tower_nd _ _ _ (flat_interp_tuple (n:=count_out)) _.
+
+Fixpoint interp_nm_expr' count_in count_out {struct count_in}
+  : (interp_all_binders_for' (Expr_nm_OpT count_in count_out) WordW.interp_base_type
+     -> interp_flat_type WordW.interp_base_type
+                         (remove_all_binders (Expr_nm_OpT count_in count_out)))
+    -> Tower.tower_nd Specific.GF25519BoundedCommon.fe25519W
+                      (interp_flat_type WordW.interp_base_type (Expr_n_OpT count_out))
+                      count_in.
+Proof.
+  refine match count_in
+               return (interp_all_binders_for' (Expr_nm_OpT count_in count_out) _
+                       -> interp_flat_type _ (remove_all_binders (Expr_nm_OpT count_in count_out)))
+                      -> Tower.tower_nd
+                           Specific.GF25519BoundedCommon.fe25519W
+                           _
+                           count_in
+         with
+         | 0 => fun e => e tt
+         | S n => fun e => let k := curry_unop_fe25519W in
+                           let v := @interp_nm_expr' n count_out in
+                           _
+         end.
+  simpl; refine (k _); clear k.
+  simpl in v, e |- *.
+  repeat (try specialize (fun x y => e (x, y));
+          let x := fresh "x" in intro x; specialize (e x)).
+  specialize (v e).
+  exact v.
+Defined.
+
+Definition interp_nm_expr'' count_in count_out (e : Expr_nm_Op count_in count_out)
+  : Tower.tower_nd Specific.GF25519BoundedCommon.fe25519W
+                   _
+                   count_in
+  := interp_nm_expr' count_in count_out (ApplyInterpedAll (Interp (@WordW.interp_op) e)).
+Definition interp_nm_expr count_in count_out (e : Expr_nm_Op count_in count_out)
+  : Tower.tower_nd Specific.GF25519BoundedCommon.fe25519W
+                   _
+                   count_in
+  := Eval cbv [interp_nm_expr'' interp_nm_expr' ApplyInterpedAll curry_unop_fe25519W Expr_nm_OpT fst snd SmartArrow fe25519T] in
+      interp_nm_expr'' count_in count_out e.
+
 Definition interp_9_4expr : Expr9_4Op
                             -> Specific.GF25519BoundedCommon.fe25519W
                             -> Specific.GF25519BoundedCommon.fe25519W
@@ -161,8 +215,21 @@ Definition interp_9_4expr : Expr9_4Op
                             -> Specific.GF25519BoundedCommon.fe25519W
                             -> Specific.GF25519BoundedCommon.fe25519W
                             -> Tuple.tuple Specific.GF25519BoundedCommon.fe25519W 4
-  := fun e => curry_9op_fe25519W (Interp (@WordW.interp_op) e).
+  := interp_nm_expr 9 4.
 
+Definition interp_bexpr : ExprBinOp -> Specific.GF25519BoundedCommon.fe25519W -> Specific.GF25519BoundedCommon.fe25519W -> Specific.GF25519BoundedCommon.fe25519W
+  := fun e => curry_binop_fe25519W (Interp (@WordW.interp_op) e).
+Definition interp_uexpr : ExprUnOp -> Specific.GF25519BoundedCommon.fe25519W -> Specific.GF25519BoundedCommon.fe25519W
+  := fun e => curry_unop_fe25519W (Interp (@WordW.interp_op) e).
+Definition interp_uexpr_FEToZ : ExprUnOpFEToZ -> Specific.GF25519BoundedCommon.fe25519W -> Specific.GF25519BoundedCommon.word64
+  := fun e => curry_unop_fe25519W (Interp (@WordW.interp_op) e).
+Definition interp_uexpr_FEToWire : ExprUnOpFEToWire -> Specific.GF25519BoundedCommon.fe25519W -> Specific.GF25519BoundedCommon.wire_digitsW
+  := fun e => curry_unop_fe25519W (Interp (@WordW.interp_op) e).
+Definition interp_uexpr_WireToFE : ExprUnOpWireToFE -> Specific.GF25519BoundedCommon.wire_digitsW -> Specific.GF25519BoundedCommon.fe25519W
+  := fun e => curry_unop_wire_digitsW (Interp (@WordW.interp_op) e).
+
+Notation nm_op_correct_and_bounded count_in count_out rop op
+  := (inm_op_correct_and_bounded count_in count_out (interp_nm_expr count_in count_out rop) (uninterp_of_tower count_in count_out op)) (only parsing).
 Notation binop_correct_and_bounded rop op
   := (ibinop_correct_and_bounded (interp_bexpr rop) op) (only parsing).
 Notation unop_correct_and_bounded rop op
@@ -194,12 +261,14 @@ Local Notation rexpr_sig T uncurried_op :=
   | interp_type_gen_rel_pointwise (fun _ => Logic.eq) (Interp interp_op (t:=T) rexprZ) uncurried_op }
     (only parsing).
 
+Notation rexpr_nm_op_sig count_in count_out op
+  := (rexpr_sig (Expr_nm_OpT count_in count_out) (interp_of_tower count_in count_out (uncurry_n_op_fe25519 count_in op))) (only parsing).
 Notation rexpr_binop_sig op := (rexpr_sig ExprBinOpT (uncurry_binop_fe25519 op)) (only parsing).
 Notation rexpr_unop_sig op := (rexpr_sig ExprUnOpT (uncurry_unop_fe25519 op)) (only parsing).
+Notation rexpr_9_4op_sig op := (rexpr_sig Expr9_4OpT (uncurry_9op_fe25519 op)) (only parsing).
 Notation rexpr_unop_FEToZ_sig op := (rexpr_sig ExprUnOpFEToZT (uncurry_unop_fe25519 op)) (only parsing).
 Notation rexpr_unop_FEToWire_sig op := (rexpr_sig ExprUnOpFEToWireT (uncurry_unop_fe25519 op)) (only parsing).
 Notation rexpr_unop_WireToFE_sig op := (rexpr_sig ExprUnOpWireToFET (uncurry_unop_wire_digits op)) (only parsing).
-Notation rexpr_9_4op_sig op := (rexpr_sig Expr9_4OpT (uncurry_9op_fe25519 op)) (only parsing).
 
 Notation correct_and_bounded_genT ropW'v ropZ_sigv
   := (let ropW' := ropW'v in
@@ -356,21 +425,70 @@ Local Ltac args_to_bounded x H :=
               | refine (fun v => match v with eq_refl => I end) ]
       ).
 
+Local Ltac eta_tuple x :=
+  let T := type of x in
+  lazymatch eval hnf in T with
+  | prod _ _ => let x0 := eta_tuple (fst x) in
+                let x1 := eta_tuple (snd x) in
+                constr:((x0, x1))
+  | _ => x
+  end.
+
 Definition unop_args_to_bounded (x : fe25519W) (H : is_bounded (fe25519WToZ x) = true)
   : interp_flat_type (fun _ => BoundedWordW.BoundedWord) (all_binders_for ExprUnOpT).
 Proof. args_to_bounded x H. Defined.
 
-Definition unopWireToFE_args_to_bounded (x : wire_digitsW) (H : wire_digits_is_bounded (wire_digitsWToZ x) = true)
-  : interp_flat_type (fun _ => BoundedWordW.BoundedWord) (all_binders_for ExprUnOpWireToFET).
-Proof. args_to_bounded x H. Defined.
+Fixpoint nm_op_args_to_bounded' pred_count_in count_out
+  : forall x : Tuple.rtuple fe25519W (S pred_count_in),
+    HList.rhlist (fun v => is_bounded (fe25519WToZ v) = true) x
+    -> interp_flat_type (fun _ => BoundedWordW.BoundedWord) (all_binders_for (Expr_nm_OpT (S pred_count_in) count_out)).
+Proof.
+  refine match pred_count_in
+               return (forall x : Tuple.rtuple fe25519W (S pred_count_in),
+                          HList.rhlist (fun v => is_bounded (fe25519WToZ v) = true) x
+                          -> interp_flat_type (fun _ => BoundedWordW.BoundedWord) (all_binders_for (Expr_nm_OpT (S pred_count_in) count_out)))
+         with
+         | 0 => unop_args_to_bounded
+         | S n
+           => fun x H
+              => let bs0 := unop_args_to_bounded (fst x) (fst H) in
+                 let bs1 := interp_all_binders_for_to'
+                              ((@nm_op_args_to_bounded' n count_out (snd x) (snd H))
+                               : @interp_all_binders_for _ (Expr_nm_OpT (S n) count_out) (fun _ => BoundedWordW.BoundedWord)) in
+                 (interp_all_binders_for_of' _ : @interp_all_binders_for _ (Expr_nm_OpT (S (S n)) count_out) (fun _ => BoundedWordW.BoundedWord))
+         end.
+  simpl in H, x |- *.
+  simpl in bs0, bs1.
+  let v := app_tuples bs0 bs1 in
+  exact v.
+Defined.
+Definition nm_op_args_to_bounded pred_count_in count_out
+  : forall x : Tuple.tuple fe25519W (S pred_count_in),
+    HList.rhlist (fun v => is_bounded (fe25519WToZ v) = true) (Tuple.assoc_right x)
+    -> interp_flat_type (fun _ => BoundedWordW.BoundedWord) (all_binders_for (Expr_nm_OpT (S pred_count_in) count_out))
+  := fun x => nm_op_args_to_bounded' pred_count_in count_out _.
+
+Declare Reduction nm_op_args_to_bounded := cbv [nm_op_args_to_bounded nm_op_args_to_bounded' interp_all_binders_for_of' interp_all_binders_for_to' Expr_nm_OpT SmartArrow fe25519T Tuple.assoc_right Tuple.assoc_right' Tuple.rsnoc' fst snd].
+
 Definition binop_args_to_bounded (x : fe25519W * fe25519W)
            (H : is_bounded (fe25519WToZ (fst x)) = true)
            (H' : is_bounded (fe25519WToZ (snd x)) = true)
-  : interp_flat_type (fun _ => BoundedWordW.BoundedWord) (all_binders_for ExprBinOpT).
-Proof.
-  let v := app_tuples (unop_args_to_bounded (fst x) H) (unop_args_to_bounded (snd x) H') in
-  exact v.
-Defined.
+  : interp_flat_type (fun _ => BoundedWordW.BoundedWord) (all_binders_for ExprBinOpT)
+  := Eval nm_op_args_to_bounded in nm_op_args_to_bounded 1 1 x (H, H').
+
+Definition op9_args_to_bounded' (x : fe25519W * fe25519W * fe25519W * fe25519W * fe25519W * fe25519W * fe25519W * fe25519W * fe25519W)
+           (H0 : is_bounded (fe25519WToZ (fst (fst (fst (fst (fst (fst (fst (fst x))))))))) = true)
+           (H1 : is_bounded (fe25519WToZ (snd (fst (fst (fst (fst (fst (fst (fst x))))))))) = true)
+           (H2 : is_bounded (fe25519WToZ (snd (fst (fst (fst (fst (fst (fst x)))))))) = true)
+           (H3 : is_bounded (fe25519WToZ (snd (fst (fst (fst (fst (fst x))))))) = true)
+           (H4 : is_bounded (fe25519WToZ (snd (fst (fst (fst (fst x)))))) = true)
+           (H5 : is_bounded (fe25519WToZ (snd (fst (fst (fst x))))) = true)
+           (H6 : is_bounded (fe25519WToZ (snd (fst (fst x)))) = true)
+           (H7 : is_bounded (fe25519WToZ (snd (fst x))) = true)
+           (H8 : is_bounded (fe25519WToZ (snd x)) = true)
+  : interp_flat_type (fun _ => BoundedWordW.BoundedWord) (all_binders_for Expr9_4OpT)
+  := Eval nm_op_args_to_bounded in nm_op_args_to_bounded 8 4 x (H0, (H1, (H2, (H3, (H4, (H5, (H6, (H7, H8)))))))).
+
 Definition op9_args_to_bounded (x : fe25519W * fe25519W * fe25519W * fe25519W * fe25519W * fe25519W * fe25519W * fe25519W * fe25519W)
            (H0 : is_bounded (fe25519WToZ (fst (fst (fst (fst (fst (fst (fst (fst x))))))))) = true)
            (H1 : is_bounded (fe25519WToZ (snd (fst (fst (fst (fst (fst (fst (fst x))))))))) = true)
@@ -395,6 +513,10 @@ Proof.
   exact v.
 Defined.
 
+Definition unopWireToFE_args_to_bounded (x : wire_digitsW) (H : wire_digits_is_bounded (wire_digitsWToZ x) = true)
+  : interp_flat_type (fun _ => BoundedWordW.BoundedWord) (all_binders_for ExprUnOpWireToFET).
+Proof. args_to_bounded x H. Defined.
+
 Local Ltac make_bounds_prop bounds orig_bounds :=
   let bounds' := fresh "bounds'" in
   let bounds_bad := fresh "bounds_bad" in
@@ -416,6 +538,29 @@ Local Ltac make_bounds_prop bounds orig_bounds :=
              | None => false
              end).
 
+Fixpoint n_op_bounds_good pred_count_out
+  : forall (bounds : interp_flat_type (fun _ => ZBounds.bounds) (remove_all_binders (Expr_n_OpT (S pred_count_out)))),
+    bool.
+Proof.
+  refine match pred_count_out
+               return interp_flat_type (fun _ => ZBounds.bounds) (remove_all_binders (Expr_n_OpT (S pred_count_out))) -> bool
+         with
+         | 0 => fun bounds => _
+         | S n => fun x => (@n_op_bounds_good n (fst x) && let bounds := snd x in _)%bool
+         end.
+  { make_bounds_prop bounds ExprUnOp_bounds. }
+  { make_bounds_prop bounds ExprUnOp_bounds. }
+Defined.
+
+Fixpoint nm_op_bounds_good count_in pred_count_out
+  : forall (bounds : interp_flat_type (fun _ => ZBounds.bounds) (remove_all_binders (Expr_nm_OpT count_in (S pred_count_out)))),
+    bool
+  := match count_in
+           return interp_flat_type (fun _ => ZBounds.bounds) (remove_all_binders (Expr_nm_OpT count_in (S pred_count_out))) -> bool
+     with
+     | 0 => n_op_bounds_good pred_count_out
+     | S n => @nm_op_bounds_good n pred_count_out
+     end.
 Definition unop_bounds_good (bounds : interp_flat_type (fun _ => ZBounds.bounds) (remove_all_binders ExprUnOpT)) : bool.
 Proof. make_bounds_prop bounds ExprUnOp_bounds. Defined.
 Definition binop_bounds_good (bounds : interp_flat_type (fun _ => ZBounds.bounds) (remove_all_binders ExprBinOpT)) : bool.
@@ -458,6 +603,18 @@ Definition ApplyUnOpFEToZ {interp_base_type var} (f : exprUnOpFEToZ interp_base_
      => LetIn (UnReturn (unop_make_args x))
               (fun k => UnReturn (Apply length_fe25519 f k)).
 
+Lemma tuple_map_flat_interp_tuple n
+      (x : interp_flat_type WordW.interp_base_type (Expr_n_OpT n))
+  : Tuple.map fe25519WToZ (flat_interp_tuple x)
+    = flat_interp_tuple (SmartVarfMap WordW.to_Z x).
+Proof.
+  destruct n as [|n]; [ reflexivity | ].
+  induction n as [|n IHn]; [ | ].
+  { destruct_head_hnf' prod; reflexivity. }
+  { destruct_head_hnf' prod.
+    simpl @flat_interp_tuple in *.
+    rewrite !Tuple.map_S, IHn; reflexivity. }
+Qed.
 
 (* FIXME TODO(jgross): This is a horrible tactic.  We should unify the
     various kinds of correct and boundedness, and abstract in Gallina
@@ -473,8 +630,9 @@ Ltac t_correct_and_bounded ropZ_sig Hbounds H0 H1 args :=
                     curry_binop_fe25519W curry_unop_fe25519W curry_unop_wire_digitsW curry_9op_fe25519W
                     curry_binop_fe25519 curry_unop_fe25519 curry_unop_wire_digits curry_9op_fe25519
                     uncurry_binop_fe25519W uncurry_unop_fe25519W uncurry_unop_wire_digitsW uncurry_9op_fe25519W
-                    uncurry_binop_fe25519 uncurry_unop_fe25519 uncurry_unop_wire_digits uncurry_9op_fe25519
-                    ExprBinOpT ExprUnOpFEToWireT ExprUnOpT ExprUnOpFEToZT ExprUnOpWireToFET Expr9_4OpT Expr4OpT
+                    uncurry_n_op_fe25519 uncurry_binop_fe25519 uncurry_unop_fe25519 uncurry_unop_wire_digits uncurry_9op_fe25519
+                    ExprBinOpT ExprUnOpFEToWireT ExprUnOpT ExprUnOpFEToZT ExprUnOpWireToFET Expr9_4OpT Expr4OpT Expr_nm_OpT
+                    uninterp_of_tower impl_under_tower_nd Expr_nm_OpT SmartArrow fe25519T interp_of_tower uncurry_n_op_fe25519 uncurry_unop_fe25519
                     interp_type_gen_rel_pointwise interp_type_gen_rel_pointwise] in *;
   cbv zeta in *;
   simpl @fe25519WToZ; simpl @wire_digitsWToZ;
@@ -506,18 +664,22 @@ Ltac t_correct_and_bounded ropZ_sig Hbounds H0 H1 args :=
   repeat match goal with x := _ |- _ => subst x end;
   cbv [id
          binop_args_to_bounded unop_args_to_bounded unopWireToFE_args_to_bounded op9_args_to_bounded
-         Relations.proj_eq_rel interp_flat_type_rel_pointwise2 SmartVarfMap interp_flat_type smart_interp_flat_map Application.all_binders_for fst snd BoundedWordW.to_wordW' BoundedWordW.boundedWordToWordW BoundedWord.value Application.ApplyInterpedAll Application.ApplyInterpedAll' Application.interp_all_binders_for_of' Application.interp_all_binders_for_to' Application.fst_binder Application.snd_binder interp_flat_type_rel_pointwise2_gen_Prop Relations.related_wordW_boundsi' Relations.related'_wordW_bounds Bounds.upper Bounds.lower Application.remove_all_binders WordW.to_Z] in Hbounds_left, Hbounds_right;
+         Relations.proj_eq_rel interp_flat_type_rel_pointwise2 SmartVarfMap interp_flat_type smart_interp_flat_map Application.all_binders_for fst snd BoundedWordW.to_wordW' BoundedWordW.boundedWordToWordW BoundedWord.value Application.ApplyInterpedAll Application.ApplyInterpedAll' Application.interp_all_binders_for_of' Application.interp_all_binders_for_to' Application.fst_binder Application.snd_binder interp_flat_type_rel_pointwise2_gen_Prop Relations.related_wordW_boundsi' Relations.related'_wordW_bounds Bounds.upper Bounds.lower Application.remove_all_binders WordW.to_Z Expr_n_OpT] in Hbounds_left, Hbounds_right;
+  cbv [Expr_n_OpT interp_nm_expr];
+  change (@Tuple.map 1) with (fun A B (f : A -> B) xs => f xs); cbv beta;
   lazymatch goal with
   | [ |- fe25519WToZ ?x = _ /\ _ ]
     => generalize dependent x; intros
   | [ |- wire_digitsWToZ ?x = _ /\ _ ]
+    => generalize dependent x; intros
+  | [ |- ((Tuple.map fe25519WToZ ?x = _) /\ _)%type ]
     => generalize dependent x; intros
   | [ |- ((Tuple.map fe25519WToZ ?x = _) * _)%type ]
     => generalize dependent x; intros
   | [ |- _ = _ ]
     => exact Hbounds_left
   end;
-  cbv [interp_type interp_type_gen interp_type_gen_hetero interp_flat_type WordW.interp_base_type remove_all_binders] in *;
+  cbv [interp_type interp_type_gen interp_type_gen_hetero interp_flat_type WordW.interp_base_type remove_all_binders Expr_n_OpT] in *;
   destruct_head' prod;
   change word64ToZ with WordW.wordWToZ in *;
   (split; [ exact Hbounds_left | ]);
@@ -555,7 +717,7 @@ Definition rword64ize {t} (x : Expr t) : Expr t
   := MapInterp (fun t => match t with TZ => word64ize end) x.
 
 Notation compute_bounds opW bounds
-  := (ApplyInterpedAll (Interp (@ZBounds.interp_op) (MapInterp (@ZBounds.of_wordW) opW)) bounds)
+  := (ApplyInterpedAll' (Interp (@ZBounds.interp_op) (MapInterp (@ZBounds.of_wordW) opW)) bounds)
        (only parsing).
 
 
